Forgot to send some files in last commit.  Now this should make completely.

theories/L1_MalechaQuoted/term.v
@@ -1,4 +1,9 @@
 
+(****)
+Add LoadPath "../common" as Common.
+Add LoadPath "../L1_MalechaQuoted" as L1.
+(****)
+
 Require Import Lists.List.
 Require Import Strings.String.
 Require Import Arith.Compare_dec.
@@ -18,6 +23,10 @@ Set Implicit Arguments.
 *** There is a special term constructor for axioms, which
 *** should be seen as having a type but no value.
 **)
+(** Assumptions:
+*** there are no nested applicatione and every application has an argument
+*** every Fixpoint has at least one function
+**)
 Inductive Term : Type :=
 | TRel       : nat -> Term
 | TSort      : Srt -> Term
@@ -33,7 +42,6 @@ Inductive Term : Type :=
 | TCase      : (nat * list nat) (* # of parameters, args per branch *) ->
                Term (* type info *) -> Term -> Terms -> Term
 | TFix       : Defs -> nat -> Term
-| TAx        : Term -> Term (* type *)
 with Terms : Type :=
 | tnil : Terms
 | tcons : Term -> Terms -> Terms
@@ -54,7 +62,26 @@ Notation set_ := (TSort SSet).
 Notation type_ := (TSort SType).
 Notation tunit t := (tcons t tnil).
 
+Fixpoint print_term (t:Term) : string :=
+  match t with
+    | TRel n => " (" ++ (nat_to_string n) ++ ") "
+    | TSort _ => " SRT "
+    | TCast _ _ _ => " CAST "
+    | TProd _ _ _ => " PROD "
+    | TLambda _ _ _ => " LAM "
+    | TLetIn _ _ _ _ => " LET "
+    | TApp fn arg args =>
+      " (APP" ++ (print_term fn) ++ (print_term arg) ++ " _ " ++ ") "
+    | TConst s => "[" ++ s ++ "]"
+    | TInd _ => " TIND "
+    | TConstruct _ n => " (CSTR " ++ (nat_to_string n) ++ ") "
+    | TCase n _ mch _ =>
+      " (CASE " ++ (nat_to_string (fst n)) ++ " _ " ++ (print_term mch) ++
+                 " _ " ++") "
+    | TFix _ n => " (FIX " ++ (nat_to_string n) ++ ") "
+  end.
 
+    
 Section TermTerms_dec. (** to make Ltac definitions local **)
 Local Ltac rght := right; injection; intuition.
 Local Ltac lft := left; subst; reflexivity.
@@ -85,14 +112,12 @@ apply TrmTrmsDefs_ind.
 - induction t; cross. destruct (inductive_dec i i0); [lft | rght].
 - induction t; cross.
   destruct (inductive_dec i i0); destruct (eq_nat_dec n n0); [lft | rght .. ].
-- induction t2; cross.
-  destruct p as [n l], p0 as [n0 l0].
-  destruct (eq_nat_dec n n0); destruct (nat_list_dec l l0);
-  destruct (H t2_1); destruct (H0 t2_2);
-  destruct (H1 t2); [lft | rght .. ].
+- induction t2; cross. destruct p as [n l], p0 as [n0 l0].
+  + destruct (eq_nat_dec n n0); destruct (nat_list_dec l l0);
+    destruct (H t2_1); destruct (H0 t2_2);
+    destruct (H1 t2); [lft | rght .. ].
 - induction t; cross.
   destruct (eq_nat_dec n n0); destruct (H d0); [lft | rght .. ].
-- induction t0; cross. destruct (H t0); [lft | rght ..].
 - induction tt; cross. lft.
 - induction tt; cross. destruct (H t1); destruct (H0 tt); [lft | rght .. ].
 - induction ee; cross. lft.
@@ -401,27 +426,14 @@ Fixpoint dlength (ts:Defs) : nat :=
     | dcons _ _ _ _ ts => S (dlength ts)
   end.
 
-Function dnthBody (n:nat) (l:Defs) {struct l} : option Term :=
+Function dnthBody (n:nat) (l:Defs) {struct l} : Term :=
   match l with
-    | dnil => None
+    | dnil => prop
     | dcons _ _ x _ t => match n with
-                           | 0 => Some x
+                           | 0 => x
                            | S m => dnthBody m t
                          end
   end.
-
-Lemma dnthBody_None: forall n ds, n >= dlength ds -> dnthBody n ds = None.
-induction n; induction ds; simpl; intuition. inversion H.
-Qed.
-
-Lemma dnthBody_Some:
-  forall ds n, n < dlength ds -> exists d, dnthBody n ds = Some d.
-induction ds; intros nx h.
-- simpl in h. inversion h.
-- destruct nx.
-  + simpl. exists t0. reflexivity.
-  + simpl. apply IHds. simpl in h. omega.
-Qed.
 
 
 (** syntactic control of "TApp": no nested apps, app must have an argument **)
@@ -638,8 +650,6 @@ Proof.
   left. intuition. revert H. not_isApp.
 - exists (TFix d n), arg, tnil. split. reflexivity.
   left. intuition. revert H. not_isApp.
-- exists (TAx fn), arg, tnil. split. reflexivity.
-  left. intuition. revert H. not_isApp.
 Qed.
 
 (** well-formed terms: TApp well-formed all the way down **)
@@ -664,7 +674,6 @@ Inductive WFapp: Term -> Prop :=
             WFapp mch -> WFapps brs -> WFapp ty ->
             WFapp (TCase m ty mch brs)
 | wfaFix: forall defs m, WFappDs defs -> WFapp (TFix defs m)
-| wfaAx: forall ty, WFapp ty -> WFapp (TAx ty)
 with WFapps: Terms -> Prop :=
 | wfanil: WFapps tnil
 | wfacons: forall t ts, WFapp t -> WFapps ts -> WFapps (tcons t ts)
@@ -743,13 +752,12 @@ Proof.
 Qed.
 
 Lemma dnthBody_pres_WFapp:
-  forall (ds:Defs), WFappDs ds -> 
-  forall n t, dnthBody n ds = Some t -> WFapp t.
+  forall (ds:Defs), WFappDs ds -> forall n, WFapp (dnthBody n ds).
 Proof.
-  intros ds h n t.
-  functional induction (dnthBody n ds); intros; try discriminate.
-  - injection H; intros; subst. inversion h. assumption.
-  - apply IHo; inversion h; assumption.
+  intros ds h n.
+  functional induction (dnthBody n ds); intros; auto.
+  - inversion h. assumption.
+  - apply IHt; inversion h; assumption.
 Qed.
 
 Lemma tskipn_pres_WFapp:
@@ -787,7 +795,6 @@ Inductive WFTrm: Term -> nat -> Prop :=
             WFTrm (TCase m ty mch brs) n
 | wfFix: forall n defs m,
            WFTrmDs defs (n + dlength defs) -> WFTrm (TFix defs m) n
-| wfAx: forall n ty, WFTrm ty n -> WFTrm (TAx ty) n
 with WFTrms: Terms -> nat -> Prop :=
 | wfnil: forall n, WFTrms tnil n
 | wfcons: forall n t ts, WFTrm t n -> WFTrms ts n -> WFTrms (tcons t ts) n
@@ -838,7 +845,6 @@ Inductive PoccTrm : Term -> Prop :=
 | PoCaseR: forall n ty mch brs, PoccTrms brs -> PoccTrm (TCase n ty mch brs)
 | PoCaseTy: forall n ty mch brs, PoccTrm ty -> PoccTrm (TCase n ty mch brs)
 | PoFix: forall ds m, PoccDefs ds -> PoccTrm (TFix ds m)
-| PoAx: forall ty, PoccTrm ty -> PoccTrm (TAx ty)
 | PoCnstr: forall m1 m2, PoccTrm (TConstruct (mkInd nm m1) m2)
 with PoccTrms : Terms -> Prop :=
 | PoThd: forall t ts, PoccTrm t -> PoccTrms (tcons t ts)
@@ -1090,9 +1096,6 @@ Proof.
     + apply PoFix. assumption.
     + apply PoAppL. apply PoFix. assumption.
   - destruct args; simpl.
-    + apply PoAx. assumption.
-    + apply PoAppL. apply PoAx. assumption.
-  - destruct args; simpl.
     + apply PoCnstr; assumption.
     + apply PoAppL. apply PoCnstr.
 Qed.
@@ -1157,8 +1160,6 @@ Inductive Instantiate: nat -> Term -> Term -> Prop :=
 | IFix: forall n d m id, 
           InstantiateDefs (n + dlength d) d id ->
           Instantiate n (TFix d m) (TFix id m)
-| IAx: forall n ty ity,
-         Instantiate n ty ity -> Instantiate n (TAx ty) (TAx ity)
 with Instantiates: nat -> Terms -> Terms -> Prop :=
 | Inil: forall n, Instantiates n tnil tnil
 | Icons: forall n t ts it its,
@@ -1217,7 +1218,6 @@ intro h. apply InstInstsDefs_ind; intros; auto.
   + apply PoCaseTy. apply H0. assumption.
 - inversion_Clear H0.
   + constructor. apply H. assumption.
-- inversion_Clear H0. constructor. intuition.
 - inversion_Clear H1.
   + constructor. apply H. assumption.
   + apply PoTtl. apply H0. assumption.
@@ -1244,7 +1244,6 @@ Function instantiate (n:nat) (tbod:Term) {struct tbod} : Term :=
     | TLetIn nm tdef ty bod =>
       TLetIn nm (instantiate n tdef) (instantiate n ty) (instantiate (S n) bod)
     | TFix ds m => TFix (instantiateDefs (n + dlength ds) ds) m
-    | TAx ty => TAx (instantiate n ty)
     | TCast t ck ty => TCast (instantiate n t) ck (instantiate n ty)
     | x => x
   end
@@ -1299,7 +1298,6 @@ apply TrmTrmsDefs_ind; intros; simpl; try (solve [constructor]).
 - apply IApp; intuition.
 - apply ICase; intuition.
 - apply IFix; intuition.
-- apply IAx. intuition.
 - apply Icons; intuition.
 - apply Idcons; intuition.
 Qed.
@@ -1380,8 +1378,6 @@ Proof.
    - change (WFapp (TFix (instantiateDefs t (n + dlength defs) defs) m)).
      constructor.
      + apply H0. assumption.
-   - change (WFapp (TAx (instantiate t n ty))).
-     constructor. apply H0. assumption.
    - change (WFapps (tcons (instantiate t0 n t) (instantiates t0 n ts))).
      constructor.
      + apply H0. assumption.
@@ -1452,7 +1448,7 @@ induction t.
 unfold whBetaStep; simpl; induction 1; intros.
 ****)
 
-Definition whCaseStep (cstrNbr:nat) (ts brs:Terms) : option Term :=
+Function whCaseStep (cstrNbr:nat) (ts brs:Terms) : option Term :=
   match tnth cstrNbr brs with
     | Some t => Some (mkApp t ts)
     | None => None
@@ -1481,23 +1477,18 @@ Definition pre_whFixStep body dts args : Term :=
              (list_to_zero (dlength dts)) body in
   (mkApp f args).
 
-Definition whFixStep (dts:Defs) (m:nat) (args:Terms) : option Term :=
-  match dnthBody m dts with
-    | Some body => Some (pre_whFixStep body dts args)
-    | None => None
-  end.
+Definition whFixStep (dts:Defs) (m:nat) (args:Terms) : Term :=
+  pre_whFixStep (dnthBody m dts) dts args.
 
 Lemma whFixStep_mkApp:
-  forall (dts:Defs) (m:nat) (args:Terms) (s:Term),
-    whFixStep dts m args = Some s -> exists f, s = mkApp f args.
+  forall (dts:Defs) (m:nat) (args:Terms),
+   exists f, whFixStep dts m args = mkApp f args.
 Proof.
-  intros dts m args s h. unfold whFixStep in h. destruct (dnthBody m dts).
-  - injection h. intros j. 
+  intros dts m args.  unfold whFixStep, pre_whFixStep.
     exists (fold_left
         (fun (bod : Term) (ndx : nat) => instantiate (TFix dts ndx) 0 bod)
-        (list_to_zero (dlength dts)) t).
-    rewrite <- j. unfold pre_whFixStep. reflexivity.
-  - discriminate.
+        (list_to_zero (dlength dts)) (dnthBody m dts)).
+    reflexivity.
 Qed.
 
 Lemma fold_left_pres_WFapp:
@@ -1513,19 +1504,15 @@ Proof.
 Qed.
 
 Lemma whFixStep_pres_WFapp:
-  forall (dts:Defs) (m:nat) (args:Terms) (s:Term),
-    WFappDs dts -> WFapps args -> whFixStep dts m args = Some s -> WFapp s.
+  forall (dts:Defs) (m:nat) (args:Terms),
+    WFappDs dts -> WFapps args -> WFapp (whFixStep dts m args).
 Proof.
-  intros dts m args s hdts hargs h.
-  unfold whFixStep in h.
-  assert (k:= dnthBody_pres_WFapp hdts m). destruct (dnthBody m dts).
-  - injection h. intros j. rewrite <- j. apply mkApp_pres_WFapp. assumption.
-    + apply fold_left_pres_WFapp.
-      * { intros. apply (proj1 instantiate_pres_WFapp). 
-          - assumption. 
-          - auto. }
-      * apply k. reflexivity.
-  - discriminate.
+  intros dts m args hdts hargs.
+  unfold whFixStep, pre_whFixStep.
+  apply mkApp_pres_WFapp. assumption.
+  apply fold_left_pres_WFapp.
+  - intros u wfu n. apply (proj1 instantiate_pres_WFapp); auto.
+  - apply (dnthBody_pres_WFapp hdts m).
 Qed.
 
 Lemma pre_whFixStep_absorbs_mkApp:
@@ -1537,13 +1524,9 @@ Proof.
 Qed.
 
 Lemma whFixStep_absorbs_mkApp:
-  forall dts m args s, whFixStep dts m args = Some s ->
-  forall brgs, exists t, whFixStep dts m (tappend args brgs) = Some t /\
-       (mkApp s brgs) = t.
+  forall dts m args brgs,
+  (mkApp (whFixStep dts m args) brgs) = (whFixStep dts m (tappend args brgs)).
 Proof.
-  unfold whFixStep. intros. destruct (dnthBody m dts); try discriminate.
-  injection H. intros h. 
-  exists (pre_whFixStep t dts (tappend args brgs)). split.
-  + reflexivity.
-  + rewrite <- h. unfold pre_whFixStep. apply mkApp_idempotent.
+  unfold whFixStep. intros.
+  rewrite (pre_whFixStep_absorbs_mkApp). reflexivity.
 Qed.
